cdcl/ConflictFunctions.fst
@@ -1,0 +1,114 @@
+module ConflictFunctions
+
+open DataTypes
+open DataTypesFunctions
+module L = FStar.List.Tot
+
+let rec backtrack_to (t : truth_assignment) (new_level : nat) : (res : truth_assignment{
+    (length res < length t)
+    /\ (forall (v : variable_info{L.contains v t && v.level <= new_level}). (L.contains v res))
+    /\ (forall (v : variable_info{L.contains v res }). (L.contains v t))
+})
+    = if length t = 0 then []
+        else
+            let x = L.hd t in
+            let temp_res = backtrack_to (L.tl t) new_level in
+                if x.level > new_level
+                then temp_res
+                else x :: temp_res
+
+let combine_clauses (cl1, cl2 : clause) 
+    : (res : clause{ 
+        (forall (lit : literal{L.contains lit cl1 || L.contains lit cl2}). (L.contains lit res)) 
+        /\ length res = length cl1 + length cl2})
+    = L.append cl1 cl2
+
+let get_smallest_level_from_new_clause (t : truth_assignment) (c : clause) : (res : nat)
+    = 
+    if length c = 0 then 0
+    else
+        let var = get_var_from_assignment t (L.hd c) in
+        let temp_res = get_smallest_level_from_new_clause t (L.tl c) in
+            if var.level < temp_res
+            then var.level
+            else temp_res
+
+let resolution (t : truth_assignment) (second_clause : clauses) (conflict_clause : clause) (guess_level : nat) (pivot : literal)
+    : (res : clause & nat) =
+    let cl1_no_pivot = remove_literal_from_list conflict_clause pivot in
+    let cl2_no_pivot = remove_literal_from_list second_clause (negate_lit pivot) in
+    let new_clause = combine_clauses cl1_no_pivot cl2_no_pivot in
+    let new_level = get_smallest_level_from_new_clause t new_clause in
+    (new_clause, new_level)
+
+let negate_clause (c : clause) : (res : clause {(length c = length res)}) =
+    let x = L.hd c in
+    (negate_lit x) :: (negate_clause (L.tl c))
+
+let intersect (#a:Type0) (l1 : list a) (l2 : list a) : (res : list a{
+    (length res <= length l1 + length l2)
+    /\ (forall (x : a{L.contains x res}). (L.contains x l1 && L.contains x l2))
+    /\ (forall (x : a{L.contains l1 && L.contains x l2}). (L.contains x res))
+})
+    =   if length l1 = 0 then []
+        else
+            let temp_res = intersect (L.tl l1) l2 in
+                if L.contains (L.hd l1) l2 
+                then (L.hd l1) :: temp_res
+                else temp_res
+
+let rec find_clause_for_resolution (f : formula) (faulty_lits : list literals) : (res : list clause & literal) =
+    if length f = 0 then []
+    else 
+        let cl = L.hd f in
+        let cls = L.tl f in
+        let common_faulty_literals = intersect faulty_literals (negate_clause cl) in
+            if length common_faulty_literals = 0
+            then find_clause_for_resolution cls faulty_literals
+            else (cl , (L.hd common_faulty_literals))
+
+//exists vars cu acel conf_level, toate din clause sunt in t
+let rec find_faulty_literals_in_conflict (t : truth_assignment) (conf_level : nat) (conflict_clause : clause) =
+    if length conflict_clause = 0 then []
+    else
+        let lit_x = L.hd conflict_clause in
+        let var_x = get_var_from_assignment t (get_literal_variable lit_x) in
+        let xs = find_faulty_literals_in_conflict t conf_level (L.tl conflict_clause) in
+            if var_x.level = conf_level
+            then lit_x :: xs
+            else xs
+
+let solve_conflict (f : formula) (t : truth_assignment {exists_conflict f t}) (current_level : nat) 
+    : (res : formula & truth_assignment & nat)
+    = let conflict_clause = get_conflict_clause f t in
+        let faulty_literals = find_faulty_literals_in_conflict t current_level conflict_clause in
+        let (clause_for_resolution, pivot) = find_clause_for_resolution f faulty_literals in
+        let (new_clause, new_level) = resolution t clause_for_resolution conflict_clause current_level pivot in
+        //am modif putin, vezi dif
+            (new_clause :: f, (backtrack_to t new_level ), new_level)
+
+val exists_conflict : formula -> truth_assignment -> bool
+let rec existsConflict f t 
+    : Tot (res : bool{ 
+        ((res = true) <==> (exists (c : clause {L.contains c f}). (is_clause_false_yet t c)))
+        /\ ((res = false) <==> (forall (c : clause{L.contains c f}). (is_clause_false_yet t c = false)))
+        }) 
+    (decreases (L.length f)) = 
+    if length f = 0
+        then false
+        else 
+            if length t = 0
+            then false
+            else
+                if is_clause_false_yet t (L.hd f) 
+                then true
+                else exists_conflict (L.tl f) t
+
+let rec get_conflict_clause 
+    (f : formula) 
+    (t : truth_assignment {exists_conflict f t = true})
+    : Tot (res : clause{L.contains res f /\ is_clause_false_yet res t = true}) 
+    (decreases (L.length f)) = 
+    if is_clause_false_yet t (L.hd f) 
+    then (L.hd f)
+    else get_conflict_clause (L.tl f) t
