cdcl/DataTypes.fst
@@ -1,0 +1,58 @@
+module DataTypes
+
+module L = FStar.List.Tot
+
+let nat_non_zero = x:int{x > 0}
+
+type literal = 
+    | Var : a: nat_non_zero -> literal
+    | NotVar : a: nat_non_zero -> literal
+    
+
+type clause = c : list literal { L.length c > 0}
+
+type variable_info = {value: bool; variable: nat_non_zero; level: nat}
+
+type formula = f : list clause 
+let empty_formula = []
+
+let rec contains_var_info (vars : list variable_info) (value : bool) (var : nat_non_zero) =
+    if L.length vars = 0 then false
+        else
+        let x = L.hd vars in
+            if x.variable = var && x.value = value
+                then true
+                else contains_var_info (L.tl vars) value var
+
+let rec count_variables_occurrence (vars: list variable_info) (v : nat_non_zero) : 
+    (res : nat {
+        ((res = 1) ==> 
+            (contains_var_info vars true v 
+                ==> (contains_var_info vars false v = false))
+            /\ (contains_var_info vars false v 
+                ==> (contains_var_info vars true v  = false)) )
+        /\ (res = 0 <==> ((contains_var_info vars true v = false)
+                        /\ (contains_var_info vars false v  = false)) )
+        /\ (res > 0 <==> ((exists (var: variable_info {List.Tot.contains var vars}). (var.variable = v)) 
+                        ) )
+     }) = if L.length vars = 0 
+            then 0
+            else let x = List.Tot.hd vars in 
+                    if x.variable = v 
+                        then let ress = count_variables_occurrence (List.Tot.tl vars) v in
+                            ress + 1
+                        else count_variables_occurrence (List.Tot.tl vars) v
+
+
+let rec ta_contition (ta : list variable_info) 
+    = (forall (var : variable_info {List.Tot.contains var ta}). 
+            ( count_variables_occurrence ta var.variable = 1 
+            ) )
+        /\ (L.length ta > 0 ==> ta_contition (List.Tot.tl ta))
+
+type truth_assignment = ta : list variable_info { ta_contition ta }
+
+type result =
+    | NotSat
+    | Sat : a: truth_assignment{ L.length a > 0} -> result
+
